First proof of [prove_handle_bind].

theories/handle_spec.v
@@ -1,4 +1,7 @@
+From Coq.Logic Require Import PropExtensionality.
 Require Import lang monads free eval handle spec.
+Set Warnings "-notation-overridden".
+Import spec.Notations.
 
 (* This file proves certain properties of [handle] in the special case
    where the target monad is [spec]. *)
@@ -7,10 +10,24 @@ Require Import lang monads free eval handle spec.
 
 (* The following notation is required for the following statement to be
    type-checked by Coq. Otherwise, the type-checker enters an infinite
-   loop. *) (* TODO *)
+   loop. *)
+
+(* TODO fix this *)
 
 Local Notation handle :=
   (@handle spec _ _ _ _).
+
+(* ------------------------------------------------------------------------ *)
+
+(* A paraphrase lemma about [handle]. *)
+
+Lemma unfold_handle {A} (m : free A) (φ : A → Prop) :
+  handle m ∋ φ ↔
+  handle_body m ∋ spec_iter_body_post handle φ.
+Proof.
+  rewrite handle_fixed_point. simpl.
+  apply descend_post. intros [|]; simpl; tauto.
+Qed.
 
 (* ------------------------------------------------------------------------ *)
 
@@ -25,52 +42,170 @@ Qed.
 
 (* ------------------------------------------------------------------------ *)
 
-(* [handle] commutes with [bind]. *)
+(* We might wish to state that [handle] commutes with [bind] in a direct
+   way, as an equality:
 
-(* In other words, [handle] is a monad morphism. *)
+   Lemma handle_bind {A B} (m : free A) (f : A → free B) :
+     handle (bind m f) =
+     bind (handle m) (λ v, handle (f v)).
 
-Lemma unfold_handle_bind {A B} (m : free A) :
-  ∀ (f : A → free B),
-  handle (bind m f) =
-  bind (handle m) (λ v, handle (f v)).
-Proof.
-  intros.
-  (* TODO set up some form of coinductive argument? *)
-  destruct m as [ | | | [ η e] k ]; intros.
-  { rewrite handle_ret.
-    do 2 rewrite bind_of_return by typeclasses eauto.
-    apply reflexivity. }
-  { rewrite bind_fail.
-    do 2 rewrite handle_fail.
-    rewrite bind_zero by typeclasses eauto.
-    apply reflexivity. }
-  { rewrite bind_next.
-    do 2 rewrite handle_next.
-    rewrite bind_zero by typeclasses eauto.
-    apply reflexivity. }
-  { rewrite bind_stop.
-    do 2 rewrite handle_stop.
-    rewrite bind_skip by typeclasses eauto.
-    rewrite <- bind_bind.
-    (* We are trying to establish something that looks like the initial goal
-       under a pair of [skip]s. *)
-    generalize (eval η e); intros m. clear η e.
-    generalize (bind m k). clear m k. intros m.
-    (* Descend under the [skip]s. *)
-    f_equal.
-    (* Apply the coinduction hypothesis. *)
-Admitted.
+   We did so in the case of the divergence monad (see handle_div.v),
+   and we were able to prove this fact via a co-inductive argument,
+   because the equality of two computations in the [div] monad is a
+   co-inductive relation.
+
+   Here, however, the equality of two inhabitants of the [spec] is
+   not co-inductively defined, so we cannot use such an argument. *)
+
+(* Instead, we split this equality into two implications, and we prove
+   one implication, arguably the most important one, the Bind rule.
+   The proof, which involves an inductive invariant, is nontrivial
+   (see below). It feels as though, to establish the Bind rule, we
+   essentially have to prove the equivalence between small-step and
+   big-step semantics. *)
+
+(* TODO think about the proof of the reverse implication;
+        think about proving both directions at once (unlikely). *)
 
 (* ------------------------------------------------------------------------ *)
 
-(* As an immediate corollary of the previous lemma, we obtain the Bind
-   rule of the program logic. That is, to reason about a sequence, it
-   suffices to reason about the left-hand side first, then to reason
-   about the right-hand side. *)
+(* The statement that we want to prove is roughly
+   that [bind (handle m) (handle f)] implies
+        [handle (bind m f)].
 
-Lemma prove_handle_bind {A B} (m : free A) (f : A → free B) (φ : B → Prop) :
+   That is, we want to prove that [handle f]
+   is able to swallow [handle m]
+   when it comes in contact with it, in front of it. *)
+
+(* To prove this fact, we must invent an invariant. This is a proof by
+   semantic co-induction: [handle] has been defined as a greatest fixed point;
+   so, to prove that [handle] holds, we must find a property that holds
+   initially and that is preserved. *)
+
+(* To express this invariant, we invent the property [stack n c φ]. This
+   property is intuitively similar to [handle c ∋ φ]: that is, it means that
+   the computation [c], transported by [handle] from the [free] monad to the
+   [spec] monad, satisfies the postcondition [φ]. However, [handle c ∋ φ] is
+   just the base case. In general, we allow the computation [c] to be a
+   sequence of [n+1] computation segments, separated by [bind]s, and the
+   specifications are chained. The specification of each segment is that it
+   eventually produces a result [a] out of which the remaining segments are
+   able to reach [φ]. *)
+
+Local Fixpoint stack {B} (n : nat) (c : free B) (φ : B → Prop) : Prop :=
+  match n with
+  | 0 =>
+      (* The base case: [c] guarantees [φ]. *)
+      handle c ∋ φ
+  | S n =>
+      (* The step case: [c] is a sequence [bind m k]
+         and [m] promises to produce a value [a]
+         out of which the remaining segments, represented by [k a],
+         guarantee [φ]. *)
+      ∃ A (m : free A) (k : A → free B),
+      c = bind m k ∧
+      handle m ∋ (λ a, stack n (k a) φ)
+  end.
+
+(* The assertion [stack n c φ] is obviously covariant in [φ]. *)
+
+Local Lemma stack_covariant {B} (φ φ' : B → Prop) :
+  (∀ a, φ a → φ' a) →
+  ∀ (n : nat) (c : free B),
+  stack n c φ →
+  stack n c φ'.
+Proof.
+  intros Hφφ'.
+  induction n; intros c; simpl.
+  { eauto using exploit_upward_closed. }
+  { intros (A & m & k & ? & Hself).
+    exists A, m, k. split; [ assumption |].
+    eapply exploit_upward_closed; [| eauto ].
+    simpl. eauto. }
+Qed.
+
+(* The invariant that we need is obtained by existentially quantifying
+   over the height [n] of the stack. *)
+
+(* [invariant] has type [free B → spec B]. *)
+
+Local Program Definition invariant {B} (c : free B) : spec B :=
+  λ (φ : B → Prop), ∃ n, stack n c φ.
+Next Obligation.
+  intros. simpl.
+  intros φ φ' Hφφ'.
+  intros (n & ?). exists n.
+  eauto using stack_covariant.
+Qed.
+
+(* [handle] is contained in this invariant. *)
+
+Local Lemma initialization {B} :
+  handle ≼ @invariant B.
+Proof.
+  (* This amounts to creating a stack of height 0. *)
+  intros i φ ?. exists 0. tauto.
+Qed.
+
+(* This invariant, which has type [free B → spec B], is preserved by
+   [spec_iter_body handle_body], a function of type
+   [(free B → spec B) → (free B → spec B)]. *)
+
+Local Lemma preservation {B} :
+  @invariant B ≼ spec_iter_body handle_body (@invariant B).
+Proof.
+  (* Put the goal into a suitable form for induction over [n]. *)
+  intros i ψ.
+  intros (n & H). revert n i ψ H.
+  (* Reduction by induction over [n]. *)
+  induction n; intros i ψ.
+  (* Base case. *)
+  { unfold stack.
+    rewrite unfold_handle.
+    rewrite unfold_spec_iter_body.
+    eapply exploit_upward_closed; intros signal.
+    eapply monotone_spec_iter_body_post.
+    eapply initialization. }
+  (* Step case. *)
+  { intros (A & m & k & ? & Hm). subst i.
+    rewrite unfold_spec_iter_body.
+    (* By cases over [m]. *)
+    destruct m as [ | | | [ η e ]].
+    { rewrite bind_of_return by typeclasses eauto.
+      rewrite handle_ret in Hm. simpl in Hm.
+      specialize (IHn _ _ Hm).
+      rewrite unfold_spec_iter_body in IHn.
+      exact IHn. }
+    { rewrite bind_fail.
+      rewrite handle_fail in Hm. simpl in Hm.
+      tauto. }
+    { rewrite bind_next.
+      rewrite handle_next in Hm. simpl in Hm.
+      tauto. }
+    { rewrite bind_stop. unfold handle_body. simpl.
+      rewrite handle_stop, unfold_skip in Hm.
+      (* Build a higher stack. *)
+      exists (S n). do 3 eexists. split; [| eauto ].
+      rewrite bind_bind. reflexivity. }
+  }
+Qed.
+
+(* Thanks to this invariant, the proof is easy. *)
+
+(* Yet, coming up with this invariant was hard. *)
+
+Lemma prove_handle_bind :
+  ∀ {A B} (m : free A) (f : A → free B) (φ : B → Prop),
   handle m ∋ (λ v, handle (f v) ∋ φ) →
   handle (bind m f) ∋ φ.
 Proof.
-  rewrite unfold_handle_bind. tauto.
+  intros A B m f φ Hm.
+  unfold handle.
+  rewrite unfold_spec_iter_preliminary.
+  exists invariant.
+  split.
+  (* Initialization. The invariant is initialized at height 1. *)
+  { exists 1. simpl. eauto. }
+  (* Preservation. *)
+  { apply preservation. }
 Qed.
